# baseURI: http://example.org/dpmm
# prefix: perse

@prefix :           <https://github.com/asteriusj/perse/> .
@prefix ex:         <http://example.org/> .
@prefix schema:     <http://schema.org/> .
@prefix rdf:        <http://www.w3.org/1999/02/22-rdf-syntax-ns#> .
@prefix owl:        <http://www.w3.org/2002/07/owl#> .
@prefix con:        <http://www.w3.org/2000/10/swap/pim/contact#> .
@prefix org:        <http://www.w3.org/ns/org#> .
@prefix vcard:      <http://www.w3.org/2006/vcard/ns#> .
@prefix bibo:	    <http://purl.org/ontology/bibo/> .
@prefix prov:       <http://www.w3.org/ns/prov#> .
@prefix obo:	    <http://purl.obolibrary.org/obo/> .
@prefix pav:	    <http://purl.org/pav/> .
@prefix prov:	    <http://www.w3.org/ns/prov#> .
@prefix sf:         <https://github.com/vocol/salesforce/> .
@prefix rdfs:       <http://www.w3.org/2000/01/rdf-schema#> .
@prefix xs:         <http://www.w3.org/2001/XMLSchema#> .
@prefix xsd:        <http://www.w3.org/2001/XMLSchema#> .
@prefix skos:       <http://www.w3.org/2004/02/skos/core#> .
@prefix sh:         <http://www.w3.org/ns/shacl#> .
@prefix foaf:       <http://xmlns.com/foaf/0.1/> .
@prefix dcterms:    <http://purl.org/dc/terms/> .
@prefix dc:         <http://purl.org/dc/elements/1.1/> .
@prefix sw:	        <http://www.w3.org/2003/06/sw-vocab-status/ns#> .
@prefix dbo:        <http://dbpedia.org/ontology/> .
@prefix vs:         <http:/s/www.w3.org/2003/06/sw-vocab-status/ns#> .
@prefix vaem:       <http://www.linkedmodel.org/schema/vaem#> .
@prefix vann:       <http://purl.org/vocab/vann/> .
@prefix perse:       <https://github.com/asteriusj/perse/> .

perse:   
        a                   owl:Ontology ;
        rdfs:comment        " Copyright (c) 2016-2018 Asterius Media LLC "@en ;
        rdfs:description    "Perse is an ontology and set of classes for creating and publishing a personalization profile with multiple facets or dimensions."@en ;
        rdfs:label          "Perse Ontology (Πέρση;)"@en ;
        dc:abstract         "An experimental ontology for defining entity relationships and data property definitions and constraints in a formal semantic representation.\n"@en ;
        dc:title            "Ontology for Perse Faceted Personalizaion Profile"@en ;
        dc:description      ""@en ;
        dc:date             "$Date: 2018-07-09 12:23:00 $" ;
        prov:generatedAtTime "$Date: 2018-07-09 12:23:006 $" ;
        dcterms:created     "$Date: 2018-02-26 20:18:26 $" ;
        dcterms:modified    "$Date: 2018-07-09 12:23:00 $" ;
        dc:creator          <http://github.com/asteriusj>;
        schema:contributor  <http://LinkedIn.com/jeffreyastewart/> , <http://github.com/asteriusj> ;
        dc:publisher        <http://github.com/asteriusj>;
        dcterms:license     "http://creativecommons.org/licenses/by/2.0/" ;
        vann:preferredNamespacePrefix
              "perse" ;
        vann:preferredNamespaceUri
              "https://github.com/asteriusj/perse#" ;
        dcterms:abstract    "\n" ;
        owl:versionIRI      "https://github.com/asteriusj/perse/Draft"@en ;
        owl:versionInfo     "Draft"@en ;
        bibo:status         "Draft"@en .

owl:Thing a owl:class ; .

skos:Concept  a             owl:Class ;
        rdfs:isDefinedBy    <http://www.w3.org/2004/02/skos/core> ;
        rdfs:label          "Concept"@en ;
        rdfs:subClassOf     owl:Thing ;
        skos:definition     "An idea or notion; a unit of thought."@en ;
        .

schema:Event  a             owl:Class ;
        rdfs:comment        "An event happening at a certain time and location, such as a concert, lecture, or festival. Ticketing information may be added via the 'offers' property. Repeated events may be structured as separate Event objects." ;
        rdfs:label          "Event"^^xsd:string ;
        rdfs:subClassOf     owl:Thing ;
        owl:equivalentClass <http://purl.org/dc/dcmitype/Event> ;
        .

foaf:Person  a              owl:Class ;
        rdfs:comment        "A person." ;
        rdfs:isDefinedBy    foaf: ;
        rdfs:label          "Person" ;
        rdfs:subClassOf     owl:Thing , <http://www.w3.org/2003/01/geo/wgs84_pos#SpatialThing> , foaf:Agent ;
        owl:disjointWith    foaf:Project , foaf:Document , foaf:Organization ;
        vs:term_status      "stable" ;
        .
        
org:Organization  a         owl:Class, rdfs:Class;
        rdfs:subClassOf     owl:Thing , foaf:Agent;
        rdfs:label          "Organization"@en;
        owl:equivalentClass foaf:Organization ;
        owl:hasKey          (org:identifier) ;
        rdfs:comment        """Represents a collection of people organized together into a community or other social, commercial or political structure. The group has some common purpose or reason for existence which goes beyond the set of people belonging to it and can act as an Agent. Organizations are often decomposable into hierarchical structures.  It is recommended that SKOS lexical labels should be used to label the Organization. In particular `skos:prefLabel` for the primary (possibly legally recognized name), `skos:altLabel` for alternative names (trading names, colloquial names) and `skos:notation` to denote a code from a code list. Alternative names: _Collective_ _Body_ _Org_ _Group_"""@en;
        rdfs:isDefinedBy    <http://www.w3.org/ns/org> ;
        .

schema:Place  a             owl:Class ;
      rdfs:label            "Place"@en;
      rdfs:subClassOf       owl:Thing ;
      rdfs:isDefinedBy      <http://schema.org/> ;
      .


## Classes

perse:Perse  a              rdfs:Class ;
        rdfs:comment        "Perse is/can be a subclass of WordNet Curriculum Vitae" ;
        dc:abstract         "Perse identifies "@en ;
        rdfs:description    ""@en ;
        rdfs:label          "Perse Profile" ;
        rdfs:subClassOf     skos:Concept ;
        dc:title            ""@en ;
        .

perse:Person  a              rdfs:Class ;
        rdfs:comment         "An object representing a single person"@en ;
        dc:abstract         "Perse Person identifies "@en ;
        rdfs:description     ""@en ;
        rdfs:label           "Person"@en ;
        rdfs:subClassOf      owl:Thing  ;
        owl:equivalentClass  <http://www.w3.org/2000/10/swap/pim/contact#Person> , dbo:Person , foaf:Person , <http://schema.org/Person> ;
        dc:title            ""@en ;
        .

perse:Organization  a        rdfs:Class ;
        rdfs:comment         "General class for organizations" ;
        rdfs:description     ""@en ;
        rdfs:label           "Organization" ;
        rdfs:subClassOf      owl:Thing ;
        dc:title             ""@en ;
        owl:equivalentClass  dbo:Organization , <http://schema.org/Organization> , foaf:Organization ;
        .


perse:Place  a              owl:Class ;
        rdfs:comment         "General class for places" ;
        rdfs:description     ""@en ;
        rdfs:label            "Place"@en;
        rdfs:subClassOf       owl:Thing ;
        rdfs:isDefinedBy      <http://schema.org/> ;
        .


## top level classes 

perse:aboutPerson  a        rdf:Property ;
        rdfs:comment        " " ;
        dc:abstract         "Perse aboutPerson identifies "@en ;
        rdfs:description    ""@en ;
        rdfs:domain         perse:Perse ;
        rdfs:label          "aboutPerson" ;
        rdfs:range          foaf:Person ;
        dc:title            ""@en ;
        .


perse:Geography  a          rdfs:Class ;
        rdfs:comment        "Def: the study of the physical features of the earth and its atmosphere, and of human activity as it affects and is affected by these, including the distribution of populations and resources, land use, and industries." ;
        dc:abstract         "Perse Geography identifies locales and geographic areas of current and historical interest." ;
        rdfs:description    "A class for Geography information."@en ;
        rdfs:label          "Geography" ;
        rdfs:subClassOf     perse:Perse ;
        dc:title            ""@en ;
        owl:equivalentClass perse:Geo ;
        .
        
        
perse:Demography  a         rdfs:Class ;
        rdfs:comment        "A class for Demography information." ;
        dc:abstract         ""@en ;
        rdfs:description    ""@en ;
        rdfs:label          "Demography" ;
        rdfs:subClassOf     perse:Perse ;
        dc:title            "Perse entry for Demography"@en ;
        .

perse:Psychography  a       rdfs:Class ;
        rdfs:comment        "Def: the study of statistics such as births, deaths, income, or the incidence of disease, which illustrate the changing structure of human populations." ;
        dc:abstract         "Perse Demography identifies "@en ;
        rdfs:description    ""@en ;
        rdfs:label          "Psychography" ;
        rdfs:subClassOf     perse:Perse ;
        dc:title            "Perse entry for Psychography"@en ;
        .

    
perse:Personality  a        rdfs:Class ;
        rdfs:comment        "Def: the combination of characteristics or qualities that form an individual's distinctive character " ;
        dc:abstract         "Perse Personality identifies "@en ;
        rdfs:description    ""@en ;
        rdfs:label          "Personality" ;
        rdfs:subClassOf     perse:Perse ;
        dc:abstract         "Perse Personality identifies " ;
        dc:title            "Perse entry for personalitys"@en ;
        .
    
    
perse:Relationship  a       rdfs:Class ;
        rdfs:comment        "Def: the way in which two or more concepts, objects, or people are connected, or the state of being connected" ;
        dc:abstract         "Perse Relationship identifies "@en ;
        rdfs:description    ""@en ;
        rdfs:label          "Relationship" ;
        rdfs:subClassOf     perse:Perse ;
        dc:abstract         "Perse Relationship identifies " ;
        dc:title            "Perse entry for relationships"@en ;
        .
        
        
perse:Experience  a         rdfs:Class ;
        rdfs:comment        "Def: practical contact with and observation of facts or events." ;
        dc:abstract         "Perse Experience identifies "@en ;
        rdfs:description    ""@en ;
        rdfs:label          "Experience" ;
        rdfs:subClassOf     perse:Perse ;
        dc:title            "Perse entry for experiences"@en ;
        .        
        
        
## second level classes



